examples/Baby.v
@@ -3,12 +3,11 @@ Require Import AutoSep.
 (** * The simplest function *)
 
 Definition diverger := bmodule "diverger" {{
-  bfunction "diverger" [SPEC reserving 0
+  bfunction "diverger"() [SPEC reserving 0
     PRE[_] [| True |]
     POST[_] [| False |] ]
-  reserving 0 {
     Diverge
-  }
+  end
 }}.
 
 (* Eval compute in compile diverger. *)
@@ -27,10 +26,9 @@ Definition immedS : spec := SPEC reserving 0
   POST[_] [| True |].
 
 Definition immed := bmodule "immed" {{
-  bfunction "immed" [immedS]
-  reserving 0 {
+  bfunction "immed"() [immedS]
     Return 0
-  }
+  end
 }}.
 
 (* Eval compute in compile immed. *)
@@ -43,50 +41,25 @@ Qed.
 
 Definition immedTest := bimport [[ "immed"!"immed" @ [immedS] ]]
   bmodule "main" {{
-    bfunction "main" [SPEC reserving 1
+    bfunction "main"() [SPEC reserving 1
       PRE[_] [| True |]
       POST[_] [| False |] ]
-    reserving 0 {
       Call "immed"!"immed"
-      [INV
+      [RET
         PRE[_] [| True |]
         POST[_] [| False |] ];;
       Diverge
-    }
+    end
   }}.
 
 (* Eval compute in compile immedTest. *)
 
 Theorem immedTestOk : moduleOk immedTest.
-  vcgen.
+  vcgen; (sep_auto; try words).
 
-  sep_auto.
-  sep_auto.
-  sep_auto.
-  sep_auto.
-  sep_auto.
-  
-Regs st Sp = Regs x Sp ^+ 4
-  H1 : Regs st Rp = Regs x Rp
-  H5 : Regs st Rv = Regs x Rv
-  H6 : interp specs
-         (![SEP.ST.star (fun (st : ST.settings) (m : smem) => x0 (st, m))
-              (SEP.ST.star (locals ("rp" :: nil) x1 1 (Regs x Sp))
-                 (SEP.ST.inj [|True|]))] (stn, st))
-  H7 : True
-  H8 : True
-  H2 : True
-  ============================
-   himp specs
-     ((fun (st0 : ST.settings) (m : smem) => x0 (st0, m)) *
-      locals ("rp" :: nil) x1 1 (Regs x Sp))%Sep
-     (SEP.ST.star (fun (stn0 : ST.settings) (sm : smem) => ?55543 (stn0, sm))
-        (locals ("rp" :: nil) ?44877 0 (Regs st Sp)))
-
-  
-  
-
-  vcgen; sep_auto.
+  (* Need to prove a theorem for switching from callee's to caller's view of stack. *)
+  instantiate (1 := fun _ => [| True |]%PropX).
+  admit.
 Qed.
 
 (* Print Assumptions immedTestOk. *)
@@ -101,47 +74,41 @@ Qed.
 
 (* Print Assumptions immedProgOk. *)
 
-Definition immedSettings := leSettings immedProg.
-Definition immedProgram := snd (labelsOf (XCAP.Blocks immedProg)).
 
-Theorem immedProgReallyOk : { w : _ | Labels immedSettings ("main", Global "main") = Some w
-  /\ forall st, safe immedSettings immedProgram (w, st) }.
-  withLabel; safety immedProgOk ("main", Global "main").
-Defined.
+(** * Incrementer *)
 
-(* Print Assumptions immedProgReallyOk. *)
+Definition incS : spec := SPEC("x") reserving 0
+  PRE[V] [| True |]
+  POST[_, rv] [| rv = V "x" ^+ $1 |].
 
-Transparent natToWord.
+Definition inc := bmodule "inc" {{
+  bfunction "inc"("x") [incS]
+    Return "x" + 1
+  end
+}}.
 
-Section final.
-  Transparent evalInstrs.
+(* Eval compute in compile inc. *)
 
-  Definition final := Eval compute in exec immedSettings immedProgram 20
-    (proj1_sig immedProgReallyOk,
-      {| Regs := fun _ => wzero _;
-        Mem := fun _ => Some (wzero _) |}).
-
-(*   Eval compute in match final with None => wzero _ | Some (_, final') => Regs final' Rp end.
-*)
-End final.
+Theorem incOk : moduleOk inc.
+  vcgen; sep_auto.
+Qed.
 
 
 (** * Always-0, in a convoluted way *)
 
-Definition always0S : assert := SPEC reserving 0
+Definition always0S : spec := SPEC("x") reserving 0
   PRE[_] [| True |]
   POST[_, rv] [| rv = $0 |].
 
 Definition always0 := bmodule "always0" {{
-  bfunction "always0" [always0S]
-  reserving 0 {
-    If (Rv = 0) {
+  bfunction "always0"("x") [always0S]
+    If ("x" = 0) {
       Skip
     } else {
-      Rv <- 0
+      "x" <- 0
     };;
-    Return Rv
-  }
+    Return "x"
+  end
 }}.
 
 (* Eval compute in compile always0. *)
